Bench/Calcite/Proven/329.lean
@@ -1,0 +1,21 @@
+import LeanDatabase.Parser
+import LeanDatabase.SQLSyntax
+open LeanDatabase Lean
+set_option maxHeartbeats 1000000
+set_option maxRecDepth 1000000
+
+namespace N_329_eq
+
+CREATE TABLE EMP («EMPNO» INT, «DEPTNO» INT, «ENAME» STRING, «JOB» STRING, «MGR» INT, «HIREDATE» INT, «SAL» INT, «COMM» INT, «SLACKER» BOOL)
+CREATE TABLE DEPT («DEPTNO» INT, «NAME» STRING)
+CREATE TABLE BONUS («ENAME» STRING, «JOB» STRING, «SAL» INT, «COMM» INT)
+CREATE TABLE EMPNULLABLES («EMPNO» INT, «DEPTNO» INT, «ENAME» STRING, «JOB» STRING, «MGR» INT, «HIREDATE» INT, «SAL» INT, «COMM» INT, «SLACKER» BOOL)
+CREATE TABLE EMPNULLABLES_20 («EMPNO» INT, «DEPTNO» INT, «ENAME» STRING, «JOB» STRING, «MGR» INT, «HIREDATE» INT, «SAL» INT, «COMM» INT, «SLACKER» BOOL)
+CREATE TABLE EMP_B («EMPNO» INT, «DEPTNO» INT, «ENAME» STRING, «JOB» STRING, «MGR» INT, «HIREDATE» INT, «SAL» INT, «COMM» INT, «SLACKER» BOOL, «BIRTHDATE» INT)
+
+theorem eq (t0 : TableRel EMP_schema) (t1 : TableRel DEPT_schema) (t2 : TableRel BONUS_schema) (t3 : TableRel EMPNULLABLES_schema) (t4 : TableRel EMPNULLABLES_20_schema) (t5 : TableRel EMP_B_schema) :
+    (sql%([EMP_schema, DEPT_schema, BONUS_schema, EMPNULLABLES_schema, EMPNULLABLES_20_schema, EMP_B_schema]) "SELECT AVG(EMP.SAL) FROM EMP, (VALUES (FALSE, TRUE, 'ab', CAST('2022-01-01' AS DATE))) AS t($f0, $f2, $f4, $f5) GROUP BY t.$f0, EMP.DEPTNO, t.$f2, EMP.EMPNO, t.$f4, t.$f5") t0 t1 t2 t3 t4 t5
+  ~= (sql%([EMP_schema, DEPT_schema, BONUS_schema, EMPNULLABLES_schema, EMPNULLABLES_20_schema, EMP_B_schema]) "SELECT AVG(EMP0.SAL) FROM EMP AS EMP0, (VALUES (FALSE, TRUE, 'ab', CAST('2022-01-01' AS DATE))) AS t3($f0, $f2, $f4, $f5) GROUP BY t3.$f0, EMP0.DEPTNO, t3.$f2, EMP0.EMPNO, t3.$f4, t3.$f5") t0 t1 t2 t3 t4 t5
+  := by sql_equiv
+
+end N_329_eq
