Bench/Literature/Problems/11_fix.lean
@@ -4,14 +4,14 @@ open LeanDatabase Lean
 set_option maxHeartbeats 1000000
 set_option maxRecDepth 1000000
 
-namespace N_11_eq
+namespace N_11_fix_eq
 
 CREATE TABLE USR («UID» INT, «UNAME» INT, «CITY» INT)
 CREATE TABLE PIC («UID» INT, «SIZE» INT)
 
 theorem eq (t0 : TableRel USR_schema) (t1 : TableRel PIC_schema) :
     (sql%([USR_schema, PIC_schema]) "SELECT X.UID AS XU, X.UNAME AS XN, (SELECT COUNT(*) AS CT FROM PIC AS Y WHERE X.UID = Y.UID AND Y.SIZE > 100000) AS CNT FROM USR AS X WHERE X.CITY = 3") t0 t1
-  ~= (sql%([USR_schema, PIC_schema]) "SELECT X.UID AS XU, X.NAME AS XN, COUNT(*) AS CNT FROM USR AS X, PIC AS Y WHERE X.UID = Y.UID AND Y.SIZE > 100000 GROUP BY X.UID, X.UNAME") t0 t1
+  ~= (sql%([USR_schema, PIC_schema]) "SELECT X.UID AS XU, X.UNAME AS XN, COUNT(*) AS CNT FROM USR AS X, PIC AS Y WHERE X.UID = Y.UID AND Y.SIZE > 100000 GROUP BY X.UID, X.UNAME") t0 t1
   := by first | sql_equiv | sorry
 
-end N_11_eq
+end N_11_fix_eq
